small_tutorial.ec
@@ -172,22 +172,22 @@ qed.
 
 module type H = { proc o () : unit }.
 
-module type Adv (H0 : H) = { proc a () : unit }.
+module type Adv (HA : H) = { proc a () : unit }.
 
 (* TODO: A: Allow the following syntax *)
 (* module (MyAdv : Adv) (H0 : H [o : `{}]) = { *)
-module (MyAdv : Adv) (H0 : H) = {
+module (MyAdv : Adv) (HA : H) = {
   proc a () = {
     var y;
-    y <- 1 + 1 + 1;
-    H0.o();
-    H0.o();
+    y <- 1 + 1 + 1 + 1;
+    HA.o();
+    HA.o();
   }
 }.
 
-lemma MyAdv_compl (k : int)(H0   <: H [o : `{k}]) : 
+lemma MyAdv_compl (k : int) (H0   <: H [o : `{k}]) : 
     choare[MyAdv(H0).a : true ==> true] 
-      time [2; H0.o : 2].
+      time [3; H0.o : 2].
 proof.
   proc; do !(call(_: true; time)); auto => /=.
 qed.
@@ -203,14 +203,14 @@ lemma MyH_compl : choare[MyH.o : true ==> true] time [1] by proc; auto.
 
 lemma advcompl_inst :
     choare[MyAdv(MyH).a : true ==> true] 
-      time [4].
+      time [5].
 proof.
   apply (MyAdv_compl 1 MyH MyH_compl). 
 qed.
 
 
-module Inv (Adv0 : Adv) (H0 : H) = {
-  module Adv1 = Adv0(H0)
+module Inv (Adv0 : Adv) (HI : H) = {
+  module Adv1 = Adv0(HI)
 
   proc i () = {
     var z;
@@ -222,14 +222,14 @@ module Inv (Adv0 : Adv) (H0 : H) = {
 
 lemma Inv_compl
     (j k h : int)
-    (Adv0 <: Adv [a : `{j, #H0.o : k}]) 
-    (H0   <: H [o : `{h}]) : 
+    (Adv0 <: Adv [a : `{j, #HA.o : k}]) 
+    (HIc   <: H [o : `{h}]) : 
     0 <= k =>
-    choare[Inv(Adv0, H0).i : true ==> true] 
-      time [1; Adv0.a : 1; H0.o : k ].
+    choare[Inv(Adv0, HIc).i : true ==> true] 
+      time [1; Adv0.a : 1; HIc.o : k ].
 proof.    
   move => hk; proc. 
-  call(_: true; time (H0.o : [fun _ => 0; H0.o : fun _ => 1])).
+  call(_: true; time (HIc.o : [fun _ => 0; HIc.o : fun _ => 1])).
   move => * /=; proc*; call(_: true; time); auto => /=.
   auto => /=.
   rewrite !big_constz !count_predT !size_range; by smt ().
@@ -237,28 +237,21 @@ qed.
 
 lemma Inv_compl_inst
     (h : int)
-    (H0   <: H [o : `{h}]) : 
-    choare[Inv(MyAdv, H0).i : true ==> true] 
-      time [1; H0.o : 2 ].
+    (H1   <: H [o : `{h}]) : 
+    choare[Inv(MyAdv, H1).i : true ==> true] 
+      time [4; H1.o : 2 ].
 proof.
-  apply (Inv_compl 2 2 1 MyAdv _ H0 _).
-
-qed.
-
-lemma invcompl2
-    (H0   <: H)
-    (Adv1 <: Adv [a : {#H0.o : 2}]) :
-    choare[Inv(Adv1, H0).i : true ==> true]
-      time [1; H0.o : 2 ].
-proof.
-  have h := (invcompl 2 Adv1 H0).
-  admit.
+  apply (Inv_compl 3 2 h MyAdv _ H1 _).
+  - apply MyAdv_compl.
+  - proc*; call(_: true; time (H1.o : [fun _ => 0; H1.o : fun _ => 1])).
+    auto; by smt(). 
 qed.
 
 (**************************************************)
 
+op kab : int.
 module type AB (H0 : H) = {
-  proc a () : unit { H0.o : 1 }
+  proc a () : unit `{ kab, H0.o : 1 }
 }.
 
 print AB.
